WIP: signed int64

theories/Universe.v
@@ -22,7 +22,15 @@ Inductive val: Type :=
 
 Definition wordsize_64 := 64.
 Definition modulus_64 := two_power_nat wordsize_64.
-Definition intrange_64 : Z -> Prop := fun z => ((- 1) < z < modulus_64)%Z.
+Definition modulus_64_half := (modulus_64 / 2)%Z.
+Definition max_64 := (modulus_64_half - 1)%Z.
+Definition min_64 := (- modulus_64_half)%Z.
+Definition intrange_64 : Z -> Prop := fun z => (min_64 <= z <= max_64)%Z.
+Definition modrange_64 : Z -> Prop := fun z => (- 1 < z < modulus_64)%Z.
+
+Ltac unfold_intrange_64 := unfold intrange_64, min_64, max_64 in *; unfold modulus_64_half, modulus_64, wordsize_64 in *.
+Ltac unfold_modrange_64 := unfold modrange_64, modulus_64, wordsize_64 in *.
+
 Definition scale_ofs (ofs : Z) := (8*ofs)%Z.
 Definition wf_val (v : val) :=
   match v with
